\documentclass[a4paper]{article}
\usepackage[left=3.5cm, right=2.5cm, top=2.5cm, bottom=2.5cm]{geometry}
\usepackage[MeX]{polski}
\usepackage[utf8]{inputenc}
\usepackage{graphicx}
\usepackage{enumerate}
\usepackage{amsmath}
\usepackage{amssymb} 
\begin{document}
$$ \sqrt{ \frac{2^{n}}{2_n}} \neq \sqrt[\frac{1}{3}]{1+n} $$
\\
$$ \frac{2^{k}}{2^{k+2}}$$
\\
$$ \frac{x^{2}}{2^{(x+2)(x-2)^{3}}}$$
\\
$$ \log_{2}{2^{8}} = 8$$
\\
$$ \sqrt[3]{e^{x}-\log_{2}{x}}$$
\\
$$\lim_{n\to\infty}\sum_{k=1}^{n}\frac{1}{k^{2}} = \frac{\pi^{2}}{6}$$
\\
$$\int_{2}^{\infty}\frac{1}{\log_2{x}dx}=\frac{1}{x}\sin x = 1 - \cos^{2}(x)$$
\\

$$\left[ \begin{array}{cccc}
a_{11} & a_{12} & \ldots &a_{1K} \\
a_{21} & a_{22} & \ldots &a_{2K}\\
\vdots & \vdots & \ddots &\vdots\\
a_{K1} & a_{K2} & \ddots & a_{KK} \\
\end{array} \right]
*
\left [\begin{array}{c}
x_{1}\\x_{2}\\\vdots \\x_{K}
\end{array} \right] =
\left [\begin{array}{c}
b_{1}\\b_{2}\\\vdots \\b_{K}
\end{array} \right]$$
\\
$$ (a_{1} = a_{1}(x)) \ \wedge\ (a_{2}=a_{2}(x)) \ \wedge \ \ldots \ \wedge \ (a_{k} = a_{k}(x)) \ \Rightarrow \ (d = d(u)) $$
\\
$$ [x]_{A} = \{y \ \in \ U :a(x) = a(y),\forall a \ \in \  A\}, \ { \rm where \  the \  control \ object \  x \in \ U } $$
\\
$$ T : [0,1] \times [0,1] \to [0,1] $$
\\
$$ \lim_{x \to \infty} \exp{(-x)} = 0$$
\\
$$
\frac{n!}{k!(n-k)!} = {n \choose k}$$
\\
$$
P\bigg(A = 2 \bigg | \frac{A^{2}}{B} > 4\bigg)$$
\\
$$ S^{C_i}(a) = \frac{(\bar{C^a_i}-\hat{C^a_i})^2}{Z_{\bar{C^a_i}^2}+Z_{\hat{C^a_i}^2}}, a \in A $$


\end{document}